unity/scheduling.lean
@@ -1,0 +1,81 @@
+
+import data.stream
+import unity.temporal
+import util.data.bijection
+
+namespace scheduling
+
+open temporal
+open classical
+
+structure fair {lbl : Type} (req : stream (set lbl)) (τ : stream lbl) : Prop :=
+  (valid : ∀ i, req i = ∅ ∨ τ i ∈ req i)
+  (fair : ∀ l, ([]<>•mem l) req → ([]<>•eq l) τ)
+
+class inductive sched (lbl : Type)
+  | fin : pos_finite lbl → sched
+  | inf : infinite lbl → sched
+
+instance nonempty_of_sched {lbl : Type} [sched lbl] : nonempty lbl := sorry
+
+lemma sched.sched {lbl : Type} : ∀ req : stream (set lbl), ∃ τ : stream lbl, fair req τ :=
+sorry
+
+instance {lbl} [i : nonempty lbl] : nonempty (stream lbl) :=
+begin
+  cases i with l,
+  apply nonempty.intro,
+  intro i, apply l,
+end
+
+noncomputable def fair_sched_of {lbl : Type} [sched lbl] (req : stream (set lbl)) : stream lbl :=
+epsilon (fair req)
+
+lemma fair_sched_of_spec {lbl : Type} [sched lbl] (req : stream (set lbl))
+: fair req (fair_sched_of req) :=
+begin
+  unfold fair_sched_of,
+  apply epsilon_spec,
+  apply sched.sched req
+end
+
+lemma fair_sched_of_mem  {lbl : Type} [sched lbl] (req : stream (set lbl))
+  (i : ℕ)
+  (Hnemp : req i ≠ ∅)
+: fair_sched_of req i ∈ req i :=
+begin
+  cases (fair_sched_of_spec req).valid i with H' H',
+  { cases Hnemp H' },
+  { apply H' }
+end
+
+lemma fair_sched_of_is_fair  {lbl : Type} [sched lbl] (req : stream (set lbl)) (l : lbl)
+: ([]<>•mem l) req → ([]<>•eq l) (fair_sched_of req) :=
+(fair_sched_of_spec req).fair l
+
+noncomputable def fair_sched (lbl : Type) [sched lbl] : stream lbl :=
+fair_sched_of (λ _ _, true)
+
+lemma fair_sched_is_fair  {lbl : Type} [sched lbl] (l : lbl)
+: ([]<>•eq l) (fair_sched lbl) :=
+begin
+  apply (fair_sched_of_spec _).fair l,
+  intro i,
+  apply eventually_weaken,
+  simp [init_drop],
+end
+
+lemma sched.sched' (lbl : Type) [sched lbl]
+: ∃ τ : stream lbl, ∀ (l : lbl), ([]<>•eq l) τ  := ⟨_,fair_sched_is_fair⟩
+
+instance fin_sched {lbl : Type} [pos_finite lbl] : sched lbl :=
+sched.fin (by apply_instance)
+
+instance inf_sched {lbl : Type} [infinite lbl] : sched lbl :=
+sched.inf (by apply_instance)
+
+instance sched_option_inf {lbl : Type} : ∀ [sched lbl], sched (option lbl)
+  | (sched.inf inf) := sched.inf (by apply_instance)
+  | (sched.fin fin) := sched.fin (by apply_instance)
+
+end scheduling
